coq/LC/Debruijn/STLC.v
@@ -1,31 +1,199 @@
 Require Import
+  Coq.Relations.Relations Coq.Relations.Relation_Operators
   Ssreflect.ssreflect Ssreflect.ssrfun Ssreflect.ssrbool Ssreflect.eqtype
   Ssreflect.ssrnat Ssreflect.seq
-  LCAC.lib.ssrnat_ext LCAC.lib.seq_ext LCAC.LC.Debruijn.Untyped.
-
-Import Lambda_tactics.
+  LCAC.lib.Relations_ext LCAC.lib.ssrnat_ext LCAC.lib.seq_ext.
 
 Set Implicit Arguments.
+Unset Strict Implicit.
+Import Prenex Implicits.
 
 Inductive typ := tyvar of nat | tyfun of typ & typ.
+Inductive term := var of nat | app of term & term & typ | abs of term.
 
 Coercion tyvar : nat >-> typ.
+Coercion var : nat >-> term.
 
-Inductive typing : context typ -> term -> typ -> Prop :=
-  | typvar ctx n ty : ctxindex ctx n ty -> typing ctx n ty
-  | typapp ctx t1 t2 ty1 ty2 :
-    typing ctx t1 (tyfun ty1 ty2) -> typing ctx t2 ty1 ->
-    typing ctx (app t1 t2) ty2
-  | typabs ctx t ty1 ty2 :
-    typing (Some ty1 :: ctx) t ty2 -> typing ctx (abs t) (tyfun ty1 ty2).
+Notation "t @[ t' \: ty ]" := (app t t' ty) (at level 60, no associativity).
 
-Hint Constructors typing.
+Fixpoint eqtyp t1 t2 :=
+  match t1, t2 with
+    | tyvar n, tyvar m => n == m
+    | tyfun t1l t1r, tyfun t2l t2r => eqtyp t1l t2l && eqtyp t1r t2r
+    | _, _ => false
+  end.
 
-Lemma typvar_seqindex ctx n ty : typing ctx (var n) ty <-> ctxindex ctx n ty.
+Lemma eqtypP : Equality.axiom eqtyp.
 Proof.
-  split => H.
-  - by inversion H.
-  - by constructor.
+  move => t1 t2; apply: (iffP idP) => [| <-].
+  - elim: t1 t2 => [n | t1l IHt1l t1r IHt1r] [m | t2l t2r] //=.
+    + by move/eqP => ->.
+    + by case/andP; move/IHt1l => ->; move/IHt1r => ->.
+  - by elim: t1 => //= t1l -> t1r.
+Defined.
+
+Canonical typ_eqMixin := EqMixin eqtypP.
+Canonical typ_eqType := Eval hnf in EqType typ typ_eqMixin.
+
+Fixpoint eqterm t1 t2 :=
+  match t1, t2 with
+    | var n, var m => n == m
+    | t1l @[t1r \: ty1], t2l @[t2r \: ty2] =>
+      [&& eqterm t1l t2l, eqterm t1r t2r & (ty1 == ty2)]
+    | abs t1, abs t2 => eqterm t1 t2
+    | _, _ => false
+  end.
+
+Lemma eqtermP : Equality.axiom eqterm.
+Proof.
+  move => t1 t2; apply: (iffP idP) => [| <-].
+  - elim: t1 t2 =>
+      [n | t1l IHt1l t1r IHt1r ty1 | t1 IHt1] [m | t2l t2r ty2 | t2] //=.
+    + by move/eqP => ->.
+    + by case/and3P; move/IHt1l => ->; move/IHt1r => ->; move/eqP => ->.
+    + by move/IHt1 => ->.
+  - by elim: t1 => //= t1l -> t1r -> /=.
+Defined.
+
+Canonical term_eqMixin := EqMixin eqtermP.
+Canonical term_eqType := Eval hnf in EqType term term_eqMixin.
+
+Fixpoint shift d c t : term :=
+  match t with
+    | var n => var (if c <= n then n + d else n)
+    | t1 @[t2 \: ty] => shift d c t1 @[shift d c t2 \: ty]
+    | abs t1 => abs (shift d c.+1 t1)
+  end.
+
+Definition substitutev ts m n : term :=
+  shift n 0 (nth (var (m - n - size ts)) ts (m - n)).
+
+Fixpoint substitute n ts t : term :=
+  match t with
+    | var m => if n <= m then substitutev ts m n else m
+    | t1 @[t2 \: ty] => substitute n ts t1 @[substitute n ts t2 \: ty]
+    | abs t' => abs (substitute n.+1 ts t')
+  end.
+
+Reserved Notation "t ->b1 t'" (at level 70, no associativity).
+
+Inductive betared1 : relation term :=
+  | betared1beta t1 t2 ty : abs t1 @[t2 \: ty] ->b1 substitute 0 [:: t2] t1
+  | betared1appl t1 t1' t2 ty :
+      t1 ->b1 t1' -> t1 @[t2 \: ty] ->b1 t1' @[t2 \: ty]
+  | betared1appr t1 t2 t2' ty :
+      t2 ->b1 t2' -> t1 @[t2 \: ty] ->b1 t1 @[t2' \: ty]
+  | betared1abs t t' : t ->b1 t' -> abs t ->b1 abs t'
+  where "t ->b1 t'" := (betared1 t t').
+
+Notation betared := [* betared1].
+Infix "->b" := betared (at level 70, no associativity).
+
+Hint Constructors betared1.
+
+Fixpoint typing (ctx : context typ) (t : term) (ty : typ) : bool :=
+  match t, ty with
+    | var n, _ => ctxindex ctx n ty
+    | tl @[tr \: ty'], _ => typing ctx tl (tyfun ty' ty) && typing ctx tr ty'
+    | abs t, tyfun tyl tyr => typing (Some tyl :: ctx) t tyr
+    | _, _ => false
+  end.
+
+Ltac elimif :=
+  (case: ifP => //=; elimif; let hyp := fresh "H" in move => hyp) || idtac.
+
+Ltac elimif_omega :=
+  elimif;
+  try (match goal with
+    | |- var _ = var _ => f_equal
+    | |- nth ?x ?xs _ = nth ?x ?xs _ => f_equal
+    | |- _ => idtac
+  end; ssromega).
+
+Lemma shiftzero n t : shift 0 n t = t.
+Proof.
+  elim: t n => /=; try congruence.
+  by move => m n; rewrite addn0 if_same.
+Qed.
+
+Lemma shift_add d d' c c' t :
+  c <= c' <= c + d -> shift d' c' (shift d c t) = shift (d' + d) c t.
+Proof.
+  case/andP; elimleq; rewrite leq_add2l; elimleq.
+  elim: t c d => /=; try (move: addSn; congruence); move => *; elimif_omega.
+Qed.
+
+Lemma shift_shift_distr d c d' c' t :
+  c' <= c -> shift d' c' (shift d c t) = shift d (d' + c) (shift d' c' t).
+Proof.
+  elimleq; elim: t c' c => /=; try (move: addSn addnS; congruence);
+    move => *; elimif_omega.
+Qed.
+
+Lemma shift_subst_distr n d c ts t :
+  c <= n -> shift d c (substitute n ts t) = substitute (d + n) ts (shift d c t).
+Proof.
+  elimleq; elim: t c n => /=; try (move: addSn addnS; congruence);
+    move => v c n; elimif_omega.
+  by rewrite /substitutev shift_add ?add0n ?leq_addr // !subnDA addnK addnA.
+Qed.
+
+Lemma subst_shift_distr n d c ts t :
+  n <= c ->
+  shift d c (substitute n ts t) =
+  substitute n (map (shift d (c - n)) ts) (shift d (size ts + c) t).
+Proof.
+  elimleq; elim: t n => /=; try (move: addnS addSn; congruence).
+  move => v n; elimif_omega; rewrite /substitutev.
+  - rewrite !nth_default ?size_map /= 1?subnAC ?subnK; elimif_omega.
+  - rewrite -shift_shift_distr // nth_map' /=.
+    f_equal; apply nth_equal; rewrite size_map; elimif_omega.
+Qed.
+
+Lemma subst_shift_cancel n d c ts t :
+  c <= n -> size ts + n <= d + c ->
+  substitute n ts (shift d c t) = shift (d - size ts) c t.
+Proof.
+  elimleq; rewrite addnAC leq_add2r; elimleq; elim: t c d => /=;
+    try (move: addSn addnS; congruence); move => v c d; elimif_omega.
+  rewrite /substitutev nth_default /=; elimif_omega.
+Qed.
+
+Lemma subst_subst_distr n m xs ys t :
+  m <= n ->
+  substitute n xs (substitute m ys t) =
+  substitute m (map (substitute (n - m) xs) ys) (substitute (size ys + n) xs t).
+Proof.
+  elimleq; elim: t m => /=; try (move: addnS addSn; congruence);
+    move => v m; elimif_omega; rewrite /substitutev.
+  - rewrite (@subst_shift_cancel m) // ?size_map; last ssromega.
+    rewrite nth_default /= /substitutev; elimif_omega.
+    by rewrite !subnDA addnK -addnA addKn (subnAC v).
+  - rewrite size_map -shift_subst_distr // nth_map' /=.
+    f_equal; apply nth_equal; rewrite size_map; elimif_omega.
+Qed.
+
+Lemma subst_app n xs ys t :
+  substitute n xs (substitute (size xs + n) ys t) = substitute n (xs ++ ys) t.
+Proof.
+  elim: t n => /=; try (move: addnS; congruence);
+    move => v n; rewrite /substitutev nth_cat size_cat; elimif_omega.
+  - by rewrite subst_shift_cancel ?addn0 // addKn addnC !subnDA.
+  - rewrite /substitutev; f_equal; apply nth_equal; ssromega.
+Qed.
+
+Lemma subst_nil n t : substitute n [::] t = t.
+Proof.
+  elim: t n => /=; try congruence; move => m n;
+    rewrite /substitutev nth_nil /=; elimif_omega.
+Qed.
+
+Lemma subst_betared1 n ts t t' :
+  t ->b1 t' -> substitute n ts t ->b1 substitute n ts t'.
+Proof.
+  move => H; move: t t' H n.
+  refine (betared1_ind _ _ _ _) => /=; auto => t t' ty n.
+  by rewrite subst_subst_distr //= add1n subn0.
 Qed.
 
 Module subject_reduction_proof.
@@ -33,65 +201,71 @@ Module subject_reduction_proof.
 Lemma ctxleq_preserves_typing ctx1 ctx2 t ty :
   ctx1 <=c ctx2 -> typing ctx1 t ty -> typing ctx2 t ty.
 Proof.
-  move => H H0; move: ctx1 t ty H0 ctx2 H.
-  refine (typing_ind _ _ _ _); eauto => ctx2 t tyl tyr H H0 ctx1 H1.
-  by constructor; apply H0; case.
+  elim: t ty ctx1 ctx2 => [n | tl IHtl tr IHtr tty | t IHt []] //=.
+  - by move => ty ctx1 ctx2; move/ctxleqP; apply.
+  - by move => ty ctx1 ctx2 H; case/andP; move/IHtl => -> //=; apply IHtr.
+  - by move => tyl tyr ctx1 ctx2 H; apply IHt; rewrite ctxleqss eqxx.
 Qed.
 
 Lemma subject_shift t ty c ctx1 ctx2 :
   typing ctx1 t ty -> typing (ctxinsert ctx2 ctx1 c) (shift (size ctx2) c t) ty.
 Proof.
-  move => H; move: ctx1 t ty H c ctx2.
-  refine (typing_ind _ _ _ _) => /=.
-  - move => ctx1 n ty H c ctx2.
-    rewrite typvar_seqindex H nth_ctxinsert; elimif_omega.
-  - eauto.
-  - move => ctx1 t ty1 ty2 H H0 c ctx2.
-    constructor; apply (H0 c.+1).
+  elim: t ty c ctx1 => [n | tl IHtl tr IHtr tty | t IHt []] //=.
+  - by move => ty c ctx1;
+      move/eqP => ->; apply/eqP; rewrite nth_ctxinsert; elimif_omega.
+  - by move => ty c ctx1; case/andP; move/IHtl => -> /=; apply IHtr.
+  - by move => tyl tyr c ctx1; apply (IHt tyr c.+1 (Some tyl :: ctx1)).
 Qed.
 
 Lemma subject_subst t ty n ctx ctx' :
-  Forall (fun p => typing (drop n ctx) p.1 p.2) ctx' ->
+  all (fun p => typing (drop n ctx) p.1 p.2) ctx' ->
   typing (ctxinsert [seq Some p.2 | p <- ctx'] ctx n) t ty ->
   typing ctx (substitute n [seq p.1 | p <- ctx'] t) ty.
-Proof with auto.
-  elim: t ty n ctx.
-  - move => /= m ty n ctx.
-    rewrite /substitutev typvar_seqindex nth_ctxinsert !size_map.
+Proof.
+  elim: t ty n ctx => [m | tl IHtl tr IHtr tty | t IHt []] //=.
+  - move => ty n ctx.
+    rewrite /substitutev nth_ctxinsert !size_map.
     elimif_omega.
-    - by constructor.
-    - move: H H0 {H1}; elimleq; rewrite ltn_add2l => H.
-      rewrite !(nth_map (var 0, tyvar 0)) // => H0 [H1]; subst.
-      case: {ctx' H H0} (nth _ _ _) (Forall_nth _ (var 0, tyvar 0) ctx' m H H0)
-        => /= t ty.
+    + move: H H0 {H1}; elimleq; rewrite ltn_add2l => H.
+      rewrite !(nth_map (var 0, tyvar 0)) // => H0; case/eqP => -> {ty}.
+      move: {H0} (all_nthP (var 0, tyvar 0) H0 m H).
       move/(subject_shift 0 (ctxinsert [::] (take n ctx) n)).
-      rewrite size_ctxinsert add0n size_take minnC minKn.
-      apply ctxleq_preserves_typing => {m t ty} m ty ->.
-      rewrite !nth_ctxinsert size_ctxinsert /=
-        size_take minnC minKn nth_nil !add0n addn0 !subn0.
-      elimif; rewrite ?nth_take ?nth_drop //; f_equal; ssromega.
-    - move => H2 H3; rewrite nth_default /=.
-      - rewrite typvar_seqindex H3; f_equal; ssromega.
-      - rewrite size_map; ssromega.
-  - move => tl IHtl tr IHtr ty n ctx H H0.
-    inversion H0; subst => /= {H0}; apply typapp with ty1...
-  - move => /= t IH ty n ctx H H0.
-    inversion H0; subst => {H0}...
+      rewrite size_ctxinsert /= add0n size_take minnC minKn /ctxinsert take0
+              sub0n take_minn minnn size_take minnE subKn ?leq_subr //=
+              drop_take_nil drop0 cats0 -catA -{4}(cat_take_drop n ctx).
+      apply ctxleq_preserves_typing.
+      rewrite ctxleq_appl.
+      case: (leqP n (size ctx)).
+      * rewrite /leq; move/eqP => -> /=; apply ctxleqxx.
+      * by move/ltnW/drop_oversize => ->; rewrite cats0 ctxleql0 size_nseq.
+    + move: H H0 {H1}; elimleq; rewrite ltn_add2l; move/negbT; rewrite -leqNgt.
+      by move => H H0 H1; rewrite nth_default /= ?size_map // addnC addnBA.
+  - by move => ty n ctx H; case/andP; move/IHtl => -> //=; apply IHtr.
+  - by move => tyl tyr n ctx H; apply (IHt tyr n.+1 (Some tyl :: ctx)).
 Qed.
+
+Lemma subject_subst0 t ty ctx ctx' :
+  all (fun p => typing ctx p.1 p.2) ctx' ->
+  typing ([seq Some p.2 | p <- ctx'] ++ ctx) t ty ->
+  typing ctx (substitute 0 [seq p.1 | p <- ctx'] t) ty.
+Proof.
+  move: (@subject_subst t ty 0 ctx ctx').
+  by rewrite /ctxinsert take0 sub0n drop0 /=.
+Qed.
+
+Arguments subject_subst [t ty n ctx] _ _ _.
+Arguments subject_subst0 [t ty ctx] _ _ _.
 
 Theorem subject_reduction ctx t1 t2 ty :
   t1 ->b1 t2 -> typing ctx t1 ty -> typing ctx t2 ty.
 Proof.
   move => H; move: t1 t2 H ctx ty.
-  refine (betared1_ind _ _ _ _ _) => //=.
-  - move => t1 t2 ctx ty H.
-    inversion H; subst; inversion H3; subst.
-    apply (subject_subst 0 ctx [:: (t2, ty1)]).
-    - by rewrite /= drop0.
-    - by rewrite /ctxinsert sub0n take0 drop0 /=.
-  - move => t1 t1' t2 H IH ctx ty H0; inversion H0; subst; eauto.
-  - move => t1 t2 t2' H IH ctx ty H0; inversion H0; subst; eauto.
-  - move => t1 t2 H IH ctx ty H0; inversion H0; subst; auto.
+  refine (betared1_ind _ _ _ _).
+  - move => /= t1 t2 tty ctx ty; case/andP => H H0.
+    by apply (subject_subst0 [:: (t2, tty)]) => //=; rewrite H0.
+  - by move => /= t1 t1' t2 tty _ IH ctx ty; case/andP; move/IH => -> ->.
+  - by move => /= t1 t2 t2' tty _ IH ctx ty; case/andP => -> /=; apply IH.
+  - move => t t' _ IH ctx [] /=; auto.
 Qed.
 
 Hint Resolve ctxleq_preserves_typing subject_subst subject_reduction.
@@ -104,27 +278,28 @@ Import subject_reduction_proof.
 
 Notation SNorm t := (Acc (fun x y => betared1 y x) t).
 
-Lemma snorm_appl tl tr : SNorm (app tl tr) -> SNorm tl.
+Lemma snorm_appl tl tr ty : SNorm (tl @[tr \: ty]) -> SNorm tl.
 Proof.
   move: tl.
   fix IH 2 => tl [H]; constructor => tl' H0.
   by apply IH, H; constructor.
-Defined.
+Qed.
 
 Fixpoint reducible (ctx : context typ) (t : term) (ty : typ) : Prop :=
   match ty with
     | tyvar n => SNorm t
     | tyfun ty1 ty2 => forall t1 ctx',
         ctx <=c ctx' -> typing ctx' t1 ty1 -> reducible ctx' t1 ty1 ->
-        reducible ctx' (app t t1) ty2
+        reducible ctx' (t @[t1 \: ty1]) ty2
   end.
 
-Definition neutral t := (if t is abs _ then False else True).
+Definition neutral t := (if t is abs _ then false else true).
 
 Lemma ctxleq_preserves_reducibility ctx ctx' t ty :
   ctx <=c ctx' -> reducible ctx t ty -> reducible ctx' t ty.
 Proof.
-  case: ty => /=; auto.
+  case: ty => //= tyl tyr H H0 t1 ctx'' H1.
+  apply H0; move: H H1; apply ctxleq_trans.
 Qed.
 
 Lemma CR2 ctx t t' ty :
@@ -133,10 +308,8 @@ Proof.
   elim: ty ctx t t'.
   - by move => /= _ _ t t' H []; apply.
   - move => /= tyl IHtyl tyr IHtyr ctx t1 t2 H H0 t3 ctx' H1 H2 H3.
-    by apply IHtyr with (app t1 t3); auto; constructor.
-Defined.
-
-Arguments CR2 [ctx t t' ty] _ _.
+    by apply IHtyr with (t1 @[t3 \: tyl]); auto.
+Qed.
 
 Hint Resolve ctxleq_preserves_reducibility CR2.
 
@@ -145,34 +318,34 @@ Lemma CR1_and_CR3 ty :
   (forall ctx t, typing ctx t ty -> neutral t ->
    (forall t', t ->b1 t' -> reducible ctx t' ty) -> reducible ctx t ty).
 Proof.
-  elim: ty.
-  - by move: Acc_intro; eauto.
-  - move => tyl [IHtyl1 IHtyl2] tyr [IHtyr1 IHtyr2] /=.
-    split => [ctx t H H0 | ctx tl H H0 H1 tr ctx' H2 H3 H4].
-    - have H1: typing (ctx ++ [:: Some tyl]) (size ctx) tyl
-        by rewrite typvar_seqindex nth_cat ltnn subnn.
-      have H2: typing (ctx ++ [:: Some tyl]) (app t (size ctx)) tyr by eauto.
-      apply snorm_appl with (size ctx), (IHtyr1 _ _ H2), IHtyr2 => // t' H3.
-      apply (CR2 H3), H0; auto.
-      apply IHtyl2 => // x H4; inversion H4.
-    - have H5: SNorm tr by apply IHtyl1 with ctx'.
-      move: tr H5 H2 H3 H4; refine (Acc_ind _ _) => tr _ IH H2 H3 H4.
-      have H5: typing ctx' (app tl tr) tyr by eauto.
-      apply IHtyr2 => // t' H6.
-      move: H0; inversion H6; subst => // _; eauto.
-Defined.
+  elim: ty; first by [].
+  move => /= tyl [IHtyl1 IHtyl2] tyr [IHtyr1 IHtyr2].
+  split => [ctx t H H0 | ctx tl H H0 H1 tr ctx' H2 H3 H4].
+  - have H1: ctxindex (ctx ++ [:: Some tyl]) (size ctx) tyl
+      by rewrite nth_cat ltnn subnn.
+    have H2: typing (ctx ++ [:: Some tyl]) (t @[size ctx \: tyl]) tyr
+      by rewrite /= H1 andbT; eauto.
+    apply snorm_appl with (size ctx) tyl, (IHtyr1 _ _ H2), IHtyr2 => // t' H3.
+    apply (CR2 H3), H0; auto.
+    apply IHtyl2 => // x H4; inversion H4.
+  - have H5: SNorm tr by apply IHtyl1 with ctx'.
+    move: tr H5 H2 H3 H4; refine (Acc_ind _ _) => tr _ IH H2 H3 H4.
+    have H5: typing ctx' (tl @[tr \: tyl]) tyr by rewrite /= H3 andbT; eauto.
+    apply IHtyr2 => // t' H6.
+    move: H0; inversion H6; subst => // _; eauto.
+Qed.
 
 Lemma CR1 ctx t ty : typing ctx t ty -> reducible ctx t ty -> SNorm t.
 Proof.
-  case: (CR1_and_CR3 ty); eauto.
-Defined.
+  case: (CR1_and_CR3 ty) => H _; apply H.
+Qed.
 
 Lemma CR3 ctx t ty :
   typing ctx t ty -> neutral t ->
   (forall t', t ->b1 t' -> reducible ctx t' ty) -> reducible ctx t ty.
 Proof.
-  case: (CR1_and_CR3 ty); auto.
-Defined.
+  case: (CR1_and_CR3 ty) => _; apply.
+Qed.
 
 Lemma snorm_subst n ts t : SNorm (substitute n ts t) -> SNorm t.
 Proof.
@@ -180,7 +353,7 @@ Proof.
   move: t3 H0 n ts t H.
   refine (Acc_ind _ _) => t3 _ IH n ts t H; subst; constructor => t' H0.
   by apply (IH (substitute n ts t') (subst_betared1 n ts H0) n ts t').
-Defined.
+Qed.
 
 Lemma abstraction_lemma ctx t1 tyl tyr :
   typing ctx (abs t1) (tyfun tyl tyr) ->
@@ -189,51 +362,52 @@ Lemma abstraction_lemma ctx t1 tyl tyr :
   reducible ctx (abs t1) (tyfun tyl tyr).
 Proof.
   move => /= H H0 t2 ctx' H1 H2 H3.
-  have H4: typing ctx' (substitute 0 [:: t2] t1) tyr by eauto.
-  move: (snorm_subst 0 [:: t2] t1 (CR1 H4 (H0 t2 ctx' H1 H2 H3)))
-    (CR1 H2 H3) => H5 H6.
+  have H4: typing ctx' (substitute 0 [:: t2] t1) tyr
+    by apply (subject_subst0 [:: (t2, tyl)]); rewrite /= ?H2 //;
+      move: H; apply ctxleq_preserves_typing; rewrite ctxleqss eqxx.
+  move: (snorm_subst (CR1 H4 (H0 t2 ctx' H1 H2 H3))) (CR1 H2 H3) => H5 H6.
   move: t1 H5 t2 H6 H H0 H1 H2 H3 {H4}.
   refine (Acc_ind _ _) => t1 H H0.
   refine (Acc_ind _ _) => t2 H1 H2 H3 H4 H5 H6 H7.
-  apply CR3 => //; eauto => t3 H8.
-  inversion H8; subst => {H8}; eauto.
-  inversion H12; subst => {H12}.
-  apply H0 => //; eauto => t'' ctx'' H8 H10 H11.
-  by apply (CR2 (subst_betared1 0 [:: t''] H9)), H4.
-Defined.
+  apply CR3 => //=.
+  - by rewrite H6 andbT; move: H3;
+      apply ctxleq_preserves_typing; rewrite ctxleqss eqxx.
+  - move => t3 H8.
+    inversion H8; subst => {H8}; eauto.
+    inversion H13; subst => {H13}.
+    apply H0 => //; eauto => t'' ctx'' H8 H10 H11.
+    by apply (CR2 (subst_betared1 0 [:: t''] H9)), H4.
+Qed.
 
 Lemma reduce_lemma ctx (ctx' : seq (term * typ)) t ty :
   typing ([seq Some p.2 | p <- ctx'] ++ ctx) t ty ->
-  Forall (fun p => typing ctx p.1 p.2 /\ reducible ctx p.1 p.2) ctx' ->
+  all (fun p => typing ctx p.1 p.2) ctx' ->
+  Forall (fun p => reducible ctx p.1 p.2) ctx' ->
   reducible ctx (substitute 0 [seq p.1 | p <- ctx'] t) ty.
 Proof.
   elim: t ty ctx ctx'.
   - move => /= n ty ctx ctx'.
-    rewrite /substitutev typvar_seqindex subn0 size_map shiftzero.
+    rewrite /substitutev subn0 size_map shiftzero.
     elim: ctx' n => [| c' ctx' IH []] /=.
-    - move => n H _; rewrite nth_nil subn0.
+    + move => n H _ _; rewrite nth_nil subn0.
       apply CR3 => //; auto => t' H0; inversion H0.
-    - move => [->]; tauto.
-    - by move => n H [_]; apply IH.
-  - move => tl IHtl tr IHtr ty ctx ctx' H H0.
-    inversion H; subst => {H}.
-    move: (IHtl (tyfun ty1 ty) ctx ctx') => /=; apply; auto.
-    apply subject_subst.
-    - rewrite drop0; move: H0; apply Forall_impl; tauto.
-    - by rewrite /ctxinsert sub0n take0 drop0 /=.
-  - move => t IHt ty ctx ctx' H H0.
-    inversion H; subst => {H} /=.
+    + move/eqP; case => ->; tauto.
+    + by move => n H; case/andP => _ H0 [_]; apply IH.
+  - move => tl IHtl tr IHtr tty ty ctx ctx' /=; case/andP => H H0 H1 H2.
+    move: (IHtl (tyfun tty ty) ctx ctx') => /=; apply; auto.
+    by apply subject_subst0.
+  - move => t IHt [] //= tyl tyr ctx ctx' H H0 H1.
     apply abstraction_lemma.
-    - apply typabs, subject_subst.
-      - rewrite /= drop0; move: H0; apply Forall_impl; tauto.
-      - by rewrite /ctxinsert /= take0 drop0 /=.
-    - move => t2 ctx2 H H1 H2.
-      rewrite subst_app.
-      apply (IHt ty2 ctx2 ((t2, ty1) :: ctx')) => /=.
-      - move: H3; apply ctxleq_preserves_typing.
-        move: H; apply (ctxleq_appl (Some ty1 :: _)).
-      - split => //; move: H0; apply Forall_impl => p []; eauto.
-Defined.
+    + rewrite -/(substitute 0 _ (abs t)).
+      by apply subject_subst0.
+    + move => t2 ctx2 H2 H3 H4.
+      rewrite subst_app /=.
+      apply (IHt tyr ctx2 ((t2, tyl) :: ctx')) => /=.
+      * move: H; apply ctxleq_preserves_typing.
+        by rewrite ctxleqss eqxx ctxleq_appl /=.
+      * apply/andP; split => //; move: H0; apply sub_all => p; eauto.
+      * split => //; move: H1; apply Forall_impl; eauto.
+Qed.
 
 Theorem typed_term_is_snorm ctx t ty : typing ctx t ty -> SNorm t.
 Proof.
@@ -241,7 +415,7 @@ Proof.
   apply (@CR1 ctx t ty) => //.
   move: (@reduce_lemma ctx [::] t ty H) => /=.
   by rewrite subst_nil; apply.
-Defined.
+Qed.
 
 End strong_normalization_proof.
 
@@ -261,11 +435,13 @@ Definition eval
 
 Module test.
 
-Goal typing [:: Some (tyvar 0)] (app (abs 0) 0) 0.
-  do !econstructor.
-Qed.
+Goal typing [:: Some (tyvar 0)] (abs 0 @[0 \: 0]) 0.
+  by [].
+Defined.
 
+(*
 Eval compute in (eval evaluation_strategies.cbn_lr Unnamed_thm).
+*)
 
 End test.
 
