coq/lib/Relations_ext.v
@@ -3,6 +3,8 @@ Require Import
   Ssreflect.ssreflect Ssreflect.ssrnat.
 
 Set Implicit Arguments.
+Unset Strict Implicit.
+Import Prenex Implicits.
 
 Notation inclusion R R' := (forall t1 t2, R t1 t2 -> R' t1 t2).
 Notation same_relation R R' := (forall t1 t2, R t1 t2 <-> R' t1 t2).
@@ -59,7 +61,7 @@ Lemma rtc_confluent A (R : relation A) : confluent R -> confluent [* R].
 Proof.
   move => H.
   apply rtc_semi_confluent.
-  move: (rtc_semi_confluent R H) => {H} H t1 t2 t3 H0 H1.
+  move: (rtc_semi_confluent H) => {H} H t1 t2 t3 H0 H1.
   by case: (H t1 t3 t2 H1 H0) => t4; case => H2 H3; exists t4.
 Qed.
 
@@ -67,9 +69,9 @@ Lemma rtc_confluent' A (R R' : relation A) :
   inclusion R R' -> inclusion R' [* R] -> confluent R' -> confluent [* R].
 Proof.
   move => H H0 H1 t1 t2 t3 H2 H3.
-  case (rtc_confluent H1 (rtc_map _ H H2) (rtc_map _ H H3))
+  case (rtc_confluent H1 (rtc_map H H2) (rtc_map H H3))
     => t4 [H4 H5].
-  by exists t4; split; rewrite -rtc_nest_elim; apply (rtc_map _ H0).
+  by exists t4; split; rewrite -rtc_nest_elim; apply (rtc_map H0).
 Qed.
 
 Theorem rtc_preservation A (P : A -> Prop) (R : relation A) :
